Makefile
@@ -64,6 +64,9 @@ ifeq (,$(NO_PULSE))
 lowparse: $(filter src/lowparse/pulse/%,$(ALL_CHECKED_FILES))
 endif
 
+lowparse-spec: $(filter src/lowparse/LowParse.Spec.%,$(ALL_CHECKED_FILES))
+.PHONY: lowparse-spec
+
 # lowparse needed because of .fst behind .fsti for extraction
 3d-prelude: $(filter src/3d/prelude/%,$(ALL_CHECKED_FILES)) $(filter-out src/lowparse/LowParse.SLow.% src/lowparse/pulse/%,$(filter src/lowparse/%,$(ALL_CHECKED_FILES)))
 	+$(MAKE) -C src/3d/prelude
